ulib/FStar.Pointer.fst
@@ -5,7 +5,6 @@ module DM = FStar.DependentMap
 module HH = FStar.HyperHeap
 module HS = FStar.HyperStack
 module HST = FStar.HyperStack.ST
-open HST // for := , !
 
 let includes_gfield_gen
   (#t: typ)
@@ -265,6 +264,7 @@ let loc_disjoint_gsub_buffer_r
 : Lemma
   (requires (UInt32.v i + UInt32.v len <= UInt32.v (buffer_length b) /\ loc_disjoint l (loc_buffer b)))
   (ensures (UInt32.v i + UInt32.v len <= UInt32.v (buffer_length b) /\ loc_disjoint l (loc_buffer (gsub_buffer b i len))))
+  [SMTPat (loc_disjoint l (loc_buffer (gsub_buffer b i len)))]
 = loc_disjoint_includes l (loc_buffer b) l (loc_buffer (gsub_buffer b i len))
 
 let loc_disjoint_gsub_buffer_l
@@ -276,6 +276,7 @@ let loc_disjoint_gsub_buffer_l
 : Lemma
   (requires (UInt32.v i + UInt32.v len <= UInt32.v (buffer_length b) /\ loc_disjoint (loc_buffer b) l))
   (ensures (UInt32.v i + UInt32.v len <= UInt32.v (buffer_length b) /\ loc_disjoint (loc_buffer (gsub_buffer b i len)) l))
+  [SMTPat (loc_disjoint (loc_buffer (gsub_buffer b i len)) l)]
 = loc_disjoint_includes (loc_buffer b) l (loc_buffer (gsub_buffer b i len)) l
 
 let loc_disjoint_addresses_pointer
@@ -363,3 +364,378 @@ let buffer_includes_gsub_r_gen
   [SMTPat (buffer_includes b0 (gsub_buffer b i len))]
 = buffer_includes_gsub_r b i len;
   buffer_includes_trans b0 b (gsub_buffer b i len)
+
+let readable_gpointer_of_buffer_cell_gsub
+  (#t: typ)
+  (h: HS.mem)
+  (b: buffer t)
+  (i: UInt32.t)
+  (len: UInt32.t)
+  (j: UInt32.t)
+: Lemma
+  (requires (
+    UInt32.v i + UInt32.v len <= UInt32.v (buffer_length b) /\
+    UInt32.v i <= UInt32.v j /\
+    UInt32.v j < UInt32.v i + UInt32.v len /\
+    buffer_readable h (gsub_buffer b i len)
+  ))
+  (ensures (
+    UInt32.v j < UInt32.v (buffer_length b) /\
+    readable h (gpointer_of_buffer_cell b j)
+  ))
+  [SMTPat (readable h (gpointer_of_buffer_cell b j)); SMTPat (buffer_readable h (gsub_buffer b i len))]
+= assert (gpointer_of_buffer_cell b j == gpointer_of_buffer_cell (gsub_buffer b i len) (UInt32.sub j i))
+
+(* buffer read: can be defined as a derived operation: pointer_of_buffer_cell ; read *)
+
+abstract
+val read_buffer
+  (#t: typ)
+  (b: buffer t)
+  (i: UInt32.t)
+: HST.Stack (type_of_typ t)
+  (requires (fun h -> UInt32.v i < UInt32.v (buffer_length b) /\ readable h (gpointer_of_buffer_cell b i)))
+  (ensures (fun h v h' -> UInt32.v i < UInt32.v (buffer_length b) /\ h' == h /\ v == Seq.index (buffer_as_seq h b) (UInt32.v i)))
+
+let read_buffer #t b i =
+  read (pointer_of_buffer_cell b i)
+
+abstract
+val write_buffer
+  (#t: typ)
+  (b: buffer t)
+  (i: UInt32.t)
+  (v: type_of_typ t)
+: HST.Stack unit
+  (requires (fun h -> UInt32.v i < UInt32.v (buffer_length b) /\ buffer_live h b))
+  (ensures (fun h _ h' ->
+    UInt32.v i < UInt32.v (buffer_length b) /\
+    modifies_1 (gpointer_of_buffer_cell b i) h h' /\
+    modifies (loc_pointer (gpointer_of_buffer_cell b i)) h h' /\
+    buffer_live h' b /\
+    readable h' (gpointer_of_buffer_cell b i) /\
+    Seq.index (buffer_as_seq h' b) (UInt32.v i) == v /\
+    (buffer_readable h b ==> (
+      buffer_readable h' b /\
+      Seq.equal (buffer_as_seq h' b) (Seq.upd (buffer_as_seq h b) (UInt32.v i) v)
+  ))))
+
+let write_buffer #t b i v =
+  let h = HST.get () in
+  write (pointer_of_buffer_cell b i) v;
+  let h' = HST.get () in
+  let f () : Lemma
+    (requires (buffer_readable h b))
+    (ensures (buffer_readable h' b))
+  = buffer_readable_intro h' b
+  in
+  Classical.move_requires f ()
+
+private
+let rec buffer_contents_equal_aux
+  (#a: typ)
+  (b1 b2: buffer a)
+  (len: UInt32.t)
+: HST.Stack bool
+  (requires (fun h ->
+    hasEq (type_of_typ a) /\
+    UInt32.v len == UInt32.v (buffer_length b1) /\
+    UInt32.v len == UInt32.v (buffer_length b2) /\
+    buffer_readable h b1 /\
+    buffer_readable h b2
+  ))
+  (ensures (fun h0 z h1 ->
+    h1 == h0 /\
+    UInt32.v len == UInt32.v (buffer_length b1) /\
+    UInt32.v len == UInt32.v (buffer_length b2) /\
+    (z == true <==> Seq.equal (buffer_as_seq h0 b1) (buffer_as_seq h0 b2))
+  ))
+  (decreases (UInt32.v len))
+= if len = 0ul
+  then true
+  else begin
+    let len' = UInt32.sub len 1ul in
+    let t : eqtype = type_of_typ a in
+    let r1 : t = read_buffer b1 len' in
+    let r2 : t = read_buffer b2 len' in
+    let b1' = sub_buffer b1 0ul len' in
+    let b2' = sub_buffer b2 0ul len' in
+    let h = HST.get () in
+    assert (Seq.equal (buffer_as_seq h b1) (Seq.snoc (buffer_as_seq h b1') r1));
+    assert (Seq.equal (buffer_as_seq h b2) (Seq.snoc (buffer_as_seq h b2') r2));
+    if r1  = r2
+    then
+      buffer_contents_equal_aux b1' b2' len'
+    else
+      false
+  end
+
+abstract
+let buffer_contents_equal
+  (#a: typ)
+  (b1 b2: buffer a)
+  (len: UInt32.t)
+: HST.Stack bool
+  (requires (fun h ->
+    hasEq (type_of_typ a) /\
+    UInt32.v len <= UInt32.v (buffer_length b1) /\
+    UInt32.v len <= UInt32.v (buffer_length b2) /\
+    buffer_readable h (gsub_buffer b1 0ul len) /\
+    buffer_readable h (gsub_buffer b2 0ul len)
+  ))
+  (ensures (fun h0 z h1 ->
+    h1 == h0 /\
+    UInt32.v len <= UInt32.v (buffer_length b1) /\
+    UInt32.v len <= UInt32.v (buffer_length b2) /\
+    (z == true <==> Seq.equal (buffer_as_seq h0 (gsub_buffer b1 0ul len)) (buffer_as_seq h0 (gsub_buffer b2 0ul len)))
+  ))
+= let b1' = sub_buffer b1 0ul len in
+  let b2' = sub_buffer b2 0ul len in
+  buffer_contents_equal_aux b1' b2' len
+
+val buffer_readable_intro_empty
+  (#t: typ)
+  (h: HS.mem)
+  (b: buffer t)
+: Lemma
+  (requires (
+    buffer_live h b /\
+    UInt32.v (buffer_length b) == 0
+  ))
+  (ensures (buffer_readable h b))
+  [SMTPatOr [
+    [SMTPat (buffer_readable h b)];
+    [SMTPat (buffer_live h b)];
+  ]]
+
+let buffer_readable_intro_empty #t h b =
+  buffer_readable_intro h b
+
+let loc_disjoint_gsub_buffer_gpointer_of_buffer_cell
+  (#a: typ)
+  (b: buffer a)
+  (i: UInt32.t)
+  (len: UInt32.t)
+  (j: UInt32.t)
+: Lemma
+  (requires (
+    UInt32.v i + UInt32.v len <= UInt32.v (buffer_length b) /\
+    UInt32.v j < UInt32.v (buffer_length b) /\
+    (UInt32.v j < UInt32.v i \/ UInt32.v i + UInt32.v len <= UInt32.v j)
+  ))
+  (ensures (
+    UInt32.v i + UInt32.v len <= UInt32.v (buffer_length b) /\
+    UInt32.v j < UInt32.v (buffer_length b) /\
+    loc_disjoint (loc_buffer (gsub_buffer b i len)) (loc_pointer (gpointer_of_buffer_cell b j))
+  ))
+  [SMTPat (loc_disjoint (loc_buffer (gsub_buffer b i len)) (loc_pointer (gpointer_of_buffer_cell b j)))]
+= assert (gpointer_of_buffer_cell b j == gpointer_of_buffer_cell (gsub_buffer b j 1ul) 0ul)
+
+private
+unfold
+let copy_buffer_contents'_pre
+  (#t: typ)
+  (a: buffer t) (* source *)
+  (b: buffer t) (* destination *)
+  (len: UInt32.t)
+  (h: HS.mem)
+: GTot Type0
+= UInt32.v len == UInt32.v (buffer_length a) /\
+  UInt32.v len == UInt32.v (buffer_length b) /\
+  buffer_readable h a /\
+  buffer_live h b /\
+  loc_disjoint (loc_buffer a) (loc_buffer b)
+
+private
+unfold
+let copy_buffer_contents'_post
+  (#t: typ)
+  (a: buffer t) (* source *)
+  (b: buffer t) (* destination *)
+  (len: UInt32.t)
+  (h0 h1: HS.mem)
+: GTot Type0
+= UInt32.v len == UInt32.v (buffer_length a) /\
+  UInt32.v len == UInt32.v (buffer_length b) /\
+  modifies (loc_buffer b) h0 h1 /\
+  buffer_readable h1 b /\
+  Seq.equal (buffer_as_seq h1 b) (buffer_as_seq h0 a)
+
+let buffer_readable_snoc
+  (#a: typ)
+  (h: HS.mem)
+  (b: buffer a)
+: Lemma
+  (requires (
+    let len = buffer_length b in (
+    UInt32.v len > 0 /\ (
+    let len' = UInt32.sub len 1ul in (
+    buffer_readable h (gsub_buffer b 0ul len') /\
+    readable h (gpointer_of_buffer_cell b len')
+  )))))
+  (ensures (
+    buffer_readable h b
+  ))
+= buffer_readable_intro h b
+
+private
+let copy_buffer_contents'_zero
+  (#t: typ)
+  (a: buffer t) (* source *)
+  (b: buffer t) (* destination *)
+  (len: UInt32.t)
+: HST.Stack unit
+  (requires (fun h ->
+    copy_buffer_contents'_pre a b len h /\
+    len == 0ul
+  ))
+  (ensures (fun h0 _ h1 ->
+    copy_buffer_contents'_post a b len h0 h1
+  ))
+= let h = HST.get () in
+  buffer_readable_intro_empty h b
+  // pattern on buffer_readable_intro_empty triggers only with the ST state AND if _pre and _post are marked `unfold`
+
+private
+let copy_buffer_contents'_nonzero
+  (#t: typ)
+  (a: buffer t) (* source *)
+  (b: buffer t) (* destination *)
+  (len: UInt32.t)
+  (h0: Ghost.erased HS.mem)
+: HST.Stack unit
+  (requires (fun h ->
+    copy_buffer_contents'_pre a b len (Ghost.reveal h0) /\
+    len <> 0ul /\ (
+    let len' = UInt32.sub len 1ul in (
+    copy_buffer_contents'_post (gsub_buffer a 0ul len') (gsub_buffer b 0ul len') len' (Ghost.reveal h0) h
+  ))))
+  (ensures (fun _ _ h1 ->
+    copy_buffer_contents'_post a b len (Ghost.reveal h0) h1
+  ))
+= let len' = UInt32.sub len 1ul in
+  let a' = sub_buffer a 0ul len' in
+  let b' = sub_buffer b 0ul len' in
+  let r = read_buffer a len' in
+  write_buffer b len' r;
+  let h1 = HST.get () in
+  buffer_readable_snoc h1 b;
+  assert (Seq.equal (buffer_as_seq h1 b) (Seq.snoc (buffer_as_seq h1 (gsub_buffer b 0ul len')) r));
+  assert (Seq.equal (buffer_as_seq (Ghost.reveal h0) a) (Seq.snoc (buffer_as_seq (Ghost.reveal h0) (gsub_buffer a 0ul len')) r))
+
+private
+let rec copy_buffer_contents'
+  (#t: typ)
+  (a: buffer t) (* source *)
+  (b: buffer t) (* destination *)
+  (len: UInt32.t)
+: HST.Stack unit
+  (requires (fun h ->
+    copy_buffer_contents'_pre a b len h
+  ))
+  (ensures (fun h0 _ h1 ->
+    copy_buffer_contents'_post a b len h0 h1
+  ))
+  (decreases (UInt32.v len))
+= if len = 0ul
+  then
+    copy_buffer_contents'_zero a b len
+  else begin
+    let _h0 = HST.get () in
+    let h0 = Ghost.hide _h0 in
+    let len' = UInt32.sub len 1ul in
+    let a' = sub_buffer a 0ul len' in
+    let b' = sub_buffer b 0ul len' in
+    copy_buffer_contents' a' b' len' ;
+    copy_buffer_contents'_nonzero a b len h0
+  end
+
+abstract
+let copy_buffer_contents
+  (#t: typ)
+  (a: buffer t) (* source *)
+  (idx_a: UInt32.t)
+  (b: buffer t) (* destination *)
+  (idx_b: UInt32.t)
+  (len: UInt32.t)
+: HST.Stack unit
+  (requires (fun h ->
+    UInt32.v idx_a + UInt32.v len <= UInt32.v (buffer_length a) /\
+    UInt32.v idx_b + UInt32.v len <= UInt32.v (buffer_length b) /\
+    buffer_live h (gsub_buffer b idx_b len) /\
+    buffer_readable h (gsub_buffer a idx_a len) /\
+    loc_disjoint (loc_buffer (gsub_buffer a idx_a len)) (loc_buffer (gsub_buffer b idx_b len))
+  ))
+  (ensures (fun h0 _ h1 ->
+    UInt32.v idx_a + UInt32.v len <= UInt32.v (buffer_length a) /\
+    UInt32.v idx_b + UInt32.v len <= UInt32.v (buffer_length b) /\
+    modifies (loc_buffer (gsub_buffer b idx_b len)) h0 h1 /\
+    buffer_readable h1 (gsub_buffer b idx_b len) /\
+    Seq.equal (buffer_as_seq h1 (gsub_buffer b idx_b len)) (buffer_as_seq h0 (gsub_buffer a idx_a len))
+  ))
+= let a' = sub_buffer a idx_a len in
+  let b' = sub_buffer b idx_b len in
+  copy_buffer_contents' a' b' len
+
+
+(*
+let h = HST.get () in
+  if len = 0ul
+  then begin
+    buffer_readable_intro_empty h b;
+    admit ()
+  end else begin
+    let len' = UInt32.sub len 1ul in
+    assert (buffer_readable h a);
+    admit ()
+  (*
+    let a' = sub_buffer a 0ul len' in
+    let h0 = HST.get () in
+    let b' = sub_buffer b 0ul len' in
+    assert (buffer_readable h0 a');
+    assert (buffer_live h0 b');
+    assert (loc_disjoint (loc_buffer a') (loc_buffer b'));
+    copy_buffer_contents' a' b' len';
+//    let r = read_buffer a len' in
+    let h05 = HST.get () in
+    assume (buffer_live h05 b);
+//    write_buffer b len' r;
+    admit ()
+    let h1 = HST.get () in
+    assume (modifies (loc_buffer b) h0 h1);
+    assume (buffer_readable h1 b);
+    assume (Seq.equal (buffer_as_seq h1 b) (buffer_as_seq h0 a))
+    *)
+  end
+
+
+(*
+
+let rec copy_buffer_contents'
+  (#t: typ)
+  (a: buffer t) (* source *)
+  (idx_a: UInt32.t)
+  (b: buffer t) (* destination *)
+  (idx_b: UInt32.t)
+  (len: UInt32.t)
+: HST.ST unit
+  (requires (fun h ->
+    UInt32.v idx_a + UInt32.v len <= UInt32.v (buffer_length a) /\
+    UInt32.v idx_b + UInt32.v len <= UInt32.v (buffer_length b) /\
+    buffer_readable h (gsub_buffer a idx_a len) /\
+    buffer_live h b /\
+    loc_disjoint (loc_buffer (gsub_buffer a idx_a len)) (loc_buffer (gsub_buffer b idx_b len))
+  ))
+  (ensures (fun h0 _ h1 ->
+    UInt32.v idx_a + UInt32.v len <= UInt32.v (buffer_length a) /\
+    UInt32.v idx_b + UInt32.v len <= UInt32.v (buffer_length b) /\
+    modifies (loc_buffer (gsub_buffer b idx_b len)) h0 h1 /\
+    buffer_readable h1 (gsub_buffer b idx_b len) /\
+    buffer_as_seq h1 (gsub_buffer b idx_b len) == buffer_as_seq h0 (gsub_buffer a idx_a len)
+  ))
+  (decreases (UInt32.v len))
+= if len = 0ul
+  then ()
+  else begin
+    
+  end
